MECMAR/spec/Notation.v
@@ -53,11 +53,14 @@ Module Notation.
   End MatchState.
   Export MatchState.Exports.
 
+  Inductive ProtoMatchResult :=
+  | SomeMS (x: MatchState)
+  | failure.
+
   (* A MatchResult is either a MatchState or the special token failure that indicates that the match failed. *)
-  Definition MatchResult := Result (option MatchState) MatchError.
+  Definition MatchResult := Result ProtoMatchResult MatchError.
   #[export]
   Instance assertion_error: Result.AssertionError MatchError := { f := AssertionFailed }.
-  Notation failure := (Success None).
   Notation out_of_fuel := (Failure OutOfFuel).
   Notation assertion_failed := (Failure AssertionFailed).
 
